tactics: fix combinators
need one for each arity... :(

ulib/FStar.Tactics.fst
@@ -112,6 +112,14 @@ let return (#a:Type) (x:a) : tactic a =
 let bind (#a:Type) (#b:Type) (t : tactic a) (f : a -> tactic b) : tactic b =
     fun () -> let r = t () in f r ()
 
+(* Fix combinator, so we need not expose the TAC effect (c.f. 1017) *)
+val fix : (tactic 'a -> tactic 'a) -> unit -> Tac 'a
+let rec fix ff (u:unit) = ff (fix ff) ()
+
+val fix1 : (('b -> tactic 'a) -> ('b -> tactic 'a)) -> 'b -> unit -> Tac 'a
+let rec fix1 ff x (u:unit) = ff (fix1 ff) x ()
+
+
 (* working around #885 *)
 let __fail (a:Type) (msg:string) : __tac a = fun s0 -> Failed #a msg s0
 let fail (#a:Type) (msg:string) : tactic a = fun () -> TAC?.reflect (__fail a msg)
